src/Analyses/Shared/Nonrelational/Abstract_Arithmetic.thy
@@ -53,6 +53,8 @@ locale expression_domain_sound =
     and pls :: "'a \<Rightarrow> 'a \<Rightarrow> 'a"
     and mns :: "'a \<Rightarrow> 'a \<Rightarrow> 'a"
     and tms :: "'a \<Rightarrow> 'a \<Rightarrow> 'a"
+    and dvs :: "'a \<Rightarrow> 'a \<Rightarrow> 'a"
+    and rem :: "'a \<Rightarrow> 'a \<Rightarrow> 'a"
     and lt :: "'a \<Rightarrow> 'a \<Rightarrow> bool option"
     and eqb :: "'a \<Rightarrow> 'a \<Rightarrow> bool option"
     and tobool :: "'a \<Rightarrow> bool option"
@@ -61,10 +63,32 @@ locale expression_domain_sound =
     and ev_Plus[simp]: "ev (Plus e1 e2) sigma = pls (ev e1 sigma) (ev e2 sigma)"
     and ev_Minus[simp]: "ev (Minus e1 e2) sigma = mns (ev e1 sigma) (ev e2 sigma)"
     and ev_Times[simp]: "ev (Times e1 e2) sigma = tms (ev e1 sigma) (ev e2 sigma)"
+    and ev_Div[simp]: "ev (Div e1 e2) sigma = dvs (ev e1 sigma) (ev e2 sigma)"
+    and ev_Mod[simp]: "ev (Mod e1 e2) sigma = rem (ev e1 sigma) (ev e2 sigma)"
     and ev_Less[simp]: "ev (Less e1 e2) sigma =
          (if is_empty (ev e1 sigma) \<or> is_empty (ev e2 sigma) then bot
           else if lt (ev e1 sigma) (ev e2 sigma) = Some True then lit 1
           else if lt (ev e1 sigma) (ev e2 sigma) = Some False then lit 0
+          else lit 0 \<squnion> lit 1)"
+    and ev_LessEq[simp]: "ev (LessEq e1 e2) sigma =
+         (if is_empty (ev e2 sigma) \<or> is_empty (ev e1 sigma) then bot
+          else if lt (ev e2 sigma) (ev e1 sigma) = Some False then lit 1
+          else if lt (ev e2 sigma) (ev e1 sigma) = Some True then lit 0
+          else lit 0 \<squnion> lit 1)"
+    and ev_Greater[simp]: "ev (Greater e1 e2) sigma =
+         (if is_empty (ev e2 sigma) \<or> is_empty (ev e1 sigma) then bot
+          else if lt (ev e2 sigma) (ev e1 sigma) = Some True then lit 1
+          else if lt (ev e2 sigma) (ev e1 sigma) = Some False then lit 0
+          else lit 0 \<squnion> lit 1)"
+    and ev_GreaterEq[simp]: "ev (GreaterEq e1 e2) sigma =
+         (if is_empty (ev e1 sigma) \<or> is_empty (ev e2 sigma) then bot
+          else if lt (ev e1 sigma) (ev e2 sigma) = Some False then lit 1
+          else if lt (ev e1 sigma) (ev e2 sigma) = Some True then lit 0
+          else lit 0 \<squnion> lit 1)"
+    and ev_NotEq[simp]: "ev (NotEq e1 e2) sigma =
+         (if is_empty (ev e1 sigma) \<or> is_empty (ev e2 sigma) then bot
+          else if eqb (ev e1 sigma) (ev e2 sigma) = Some False then lit 1
+          else if eqb (ev e1 sigma) (ev e2 sigma) = Some True then lit 0
           else lit 0 \<squnion> lit 1)"
     and ev_Eq[simp]: "ev (exp.Eq e1 e2) sigma =
          (if is_empty (ev e1 sigma) \<or> is_empty (ev e2 sigma) then bot
@@ -97,6 +121,10 @@ locale expression_domain_sound =
       "i \<in> gamma (p::'a) \<Longrightarrow> j \<in> gamma q \<Longrightarrow> i - j \<in> gamma (mns p q)"
     and times_sound[intro]:
       "i \<in> gamma (p::'a) \<Longrightarrow> j \<in> gamma q \<Longrightarrow> i * j \<in> gamma (tms p q)"
+    and div_sound[intro]:
+      "i \<in> gamma (p::'a) \<Longrightarrow> j \<in> gamma q \<Longrightarrow> c_div i j \<in> gamma (dvs p q)"
+    and mod_sound[intro]:
+      "i \<in> gamma (p::'a) \<Longrightarrow> j \<in> gamma q \<Longrightarrow> c_mod i j \<in> gamma (rem p q)"
     and lt_sound: "lt p q = Some b \<Longrightarrow> i \<in> gamma (p::'a) \<Longrightarrow> j \<in> gamma q \<Longrightarrow> (i < j) = b"
     and eqb_sound: "eqb p q = Some b \<Longrightarrow> i \<in> gamma (p::'a) \<Longrightarrow> j \<in> gamma q \<Longrightarrow> (i = j) = b"
     and tobool_sound: "tobool p = Some b \<Longrightarrow> i \<in> gamma (p::'a) \<Longrightarrow> truthy i = b"
@@ -124,7 +152,33 @@ proof (induction a arbitrary: s sigma)
   show ?case unfolding ev_Less aval.simps
     by (rule bool_lit_sound) (use h1 h2 is_empty_correct lt_sound[OF _ h1 h2] in auto)
 next
-  case (Eq e1 e2)
+
+  case (LessEq e1 e2)
+  have h1: "aval e1 s \<in> gamma (ev e1 sigma)" and h2: "aval e2 s \<in> gamma (ev e2 sigma)"
+    using LessEq by simp_all
+  show ?case unfolding ev_LessEq aval.simps
+    by (rule bool_lit_sound) (use h1 h2 is_empty_correct lt_sound[where b=True, OF _ h2 h1]
+        lt_sound[where b=False, OF _ h2 h1] in auto)
+next
+  case (Greater e1 e2)
+  have h1: "aval e1 s \<in> gamma (ev e1 sigma)" and h2: "aval e2 s \<in> gamma (ev e2 sigma)"
+    using Greater by simp_all
+  show ?case unfolding ev_Greater aval.simps
+    by (rule bool_lit_sound) (use h1 h2 is_empty_correct lt_sound[OF _ h2 h1] in auto)
+next
+  case (GreaterEq e1 e2)
+  have h1: "aval e1 s \<in> gamma (ev e1 sigma)" and h2: "aval e2 s \<in> gamma (ev e2 sigma)"
+    using GreaterEq by simp_all
+  show ?case unfolding ev_GreaterEq aval.simps
+    by (rule bool_lit_sound) (use h1 h2 is_empty_correct lt_sound[where b=True, OF _ h1 h2]
+        lt_sound[where b=False, OF _ h1 h2] in auto)
+next
+  case (NotEq e1 e2)
+  have h1: "aval e1 s \<in> gamma (ev e1 sigma)" and h2: "aval e2 s \<in> gamma (ev e2 sigma)"
+    using NotEq by simp_all
+  show ?case unfolding ev_NotEq aval.simps
+    by (rule bool_lit_sound) (use h1 h2 is_empty_correct eqb_sound[OF _ h1 h2] in auto)
+next  case (Eq e1 e2)
   have h1: "aval e1 s \<in> gamma (ev e1 sigma)" and h2: "aval e2 s \<in> gamma (ev e2 sigma)"
     using Eq by simp_all
   show ?case unfolding ev_Eq aval.simps
@@ -169,6 +223,10 @@ locale expression_domain_mono = expression_domain_sound +
       "p1 \<le> p2 \<Longrightarrow> q1 \<le> q2 \<Longrightarrow> mns p1 q1 \<le> mns p2 q2"
     and times_mono[intro]:
       "p1 \<le> p2 \<Longrightarrow> q1 \<le> q2 \<Longrightarrow> tms p1 q1 \<le> tms p2 q2"
+    and div_mono[intro]:
+      "p1 \<le> p2 \<Longrightarrow> q1 \<le> q2 \<Longrightarrow> dvs p1 q1 \<le> dvs p2 q2"
+    and mod_mono[intro]:
+      "p1 \<le> p2 \<Longrightarrow> q1 \<le> q2 \<Longrightarrow> rem p1 q1 \<le> rem p2 q2"
     and lt_mono:
       "\<not> is_empty p1 \<Longrightarrow> \<not> is_empty q1 \<Longrightarrow> p1 \<le> p2 \<Longrightarrow> q1 \<le> q2 \<Longrightarrow>
        lt p2 q2 = Some b \<Longrightarrow> lt p1 q1 = Some b"
@@ -196,7 +254,35 @@ proof (induction a arbitrary: sigma1 sigma2)
     by (rule bool_lit_mono)
        (use is_empty_antimono[OF p] is_empty_antimono[OF q] lt_mono[OF _ _ p q] in auto)
 next
-  case (Eq e1 e2)
+
+  case (LessEq e1 e2)
+  have p: "ev e1 sigma1 \<le> ev e1 sigma2" and q: "ev e2 sigma1 \<le> ev e2 sigma2"
+    using LessEq by simp_all
+  show ?case unfolding ev_LessEq
+    by (rule bool_lit_mono)
+       (use is_empty_antimono[OF p] is_empty_antimono[OF q] lt_mono[OF _ _ q p] in auto)
+next
+  case (Greater e1 e2)
+  have p: "ev e1 sigma1 \<le> ev e1 sigma2" and q: "ev e2 sigma1 \<le> ev e2 sigma2"
+    using Greater by simp_all
+  show ?case unfolding ev_Greater
+    by (rule bool_lit_mono)
+       (use is_empty_antimono[OF p] is_empty_antimono[OF q] lt_mono[OF _ _ q p] in auto)
+next
+  case (GreaterEq e1 e2)
+  have p: "ev e1 sigma1 \<le> ev e1 sigma2" and q: "ev e2 sigma1 \<le> ev e2 sigma2"
+    using GreaterEq by simp_all
+  show ?case unfolding ev_GreaterEq
+    by (rule bool_lit_mono)
+       (use is_empty_antimono[OF p] is_empty_antimono[OF q] lt_mono[OF _ _ p q] in auto)
+next
+  case (NotEq e1 e2)
+  have p: "ev e1 sigma1 \<le> ev e1 sigma2" and q: "ev e2 sigma1 \<le> ev e2 sigma2"
+    using NotEq by simp_all
+  show ?case unfolding ev_NotEq
+    by (rule bool_lit_mono)
+       (use is_empty_antimono[OF p] is_empty_antimono[OF q] eqb_mono[OF _ _ p q] in auto)
+next  case (Eq e1 e2)
   have p: "ev e1 sigma1 \<le> ev e1 sigma2" and q: "ev e2 sigma1 \<le> ev e2 sigma2"
     using Eq by simp_all
   show ?case unfolding ev_Eq
